Clean/Tables/KeccakInductive.lean
@@ -16,7 +16,7 @@ def table : InductiveTable (F p) KeccakState KeccakBlock where
 
   Spec i state blocks _ : Prop :=
     state.Normalized
-    ∧ state.value = absorb_blocks (blocks.map KeccakBlock.value)
+    ∧ state.value = absorbBlocks (blocks.map KeccakBlock.value)
 
   input_assumptions i block := block.Normalized
 
@@ -24,7 +24,7 @@ def table : InductiveTable (F p) KeccakState KeccakBlock where
     intro i env state_var block_var state block blocks _ h_input h_holds spec_previous
     simp_all only [circuit_norm, subcircuit_norm,
       AbsorbBlock.circuit, AbsorbBlock.Assumptions, AbsorbBlock.Spec,
-      KeccakBlock.normalized, absorb_blocks]
+      KeccakBlock.normalized, absorbBlocks]
     rw [List.concat_eq_append, List.map_append, List.map_cons, List.map_nil, List.foldl_concat]
 
   completeness := by
@@ -48,13 +48,13 @@ def formalTable (output : KeccakState (F p)) := table.toFormal initialState outp
 -- The table's statement implies that the output state is the result of keccak-hashing some list of input blocks
 theorem tableStatement (output : KeccakState (F p)) : ∀ n > 0, ∀ trace, ∃ blocks, blocks.length = n - 1 ∧
   (formalTable output).statement n trace →
-    output.Normalized ∧ output.value = absorb_blocks blocks := by
+    output.Normalized ∧ output.value = absorbBlocks blocks := by
   intro n hn trace
   use (InductiveTable.traceInputs trace.tail).map KeccakBlock.value
   intro Spec
   simp only [formalTable, FormalTable.statement, table, InductiveTable.toFormal] at Spec
   simp only [List.length_map, Trace.toList_length, trace.tail.prop, InductiveTable.traceInputs, hn] at Spec
-  simp only [initialState_value, initialState_normalized, absorb_blocks, initial_state, true_and] at Spec
+  simp only [initialState_value, initialState_normalized, absorbBlocks, Specs.Keccak256.initialState, true_and] at Spec
   exact Spec rfl
 
 end Tables.KeccakInductive
